theories/elpi_equiv.v
@@ -7,36 +7,33 @@ Section NurEqiv.
   Variable (u : Unif).
   Variable (p : program).
 
-  Lemma tree_to_elpi fv A s1 B s2 b s0 fv':
+  Lemma tree_to_elpi fv A s1 B sF b s0 fv':
     vars_tree A `<=` fv -> vars_sigma s1 `<=` fv ->
     valid_tree A ->
-      run u p fv s1 A (Some s2) B b fv' -> 
+      run u p fv s1 A (Some sF) B b fv' -> 
         exists x xs,
           t2l A s1 nilC = x ::: xs /\
-          nur u p fv x.1 x.2 xs s2 (t2l (odflt KO B) s0 nilC).
+          nur u p fv x.1 x.2 xs sF (t2l (odflt KO B) s0 nilC).
   Proof.
     move=> +++H.
     remember (Some _) as r eqn:Hr.
-    elim: H s2 Hr s0; clear => //.
-    + move=> s1 _ A _ sA fv <-<- _ [<-] sIgn fvP fvP' vA; subst.
-      rewrite (success_t2l sIgn)//.
+    elim_run H sF Hr s0 => vtA vts1 vA.
+    + move: Hr => [?]; subst.
+      rewrite (success_t2l s0)//.
       repeat eexists.
       apply: StopE.
-    + move=> s1 s2 r A B n fv fv' ? eA rB IH s4 ? sIgn fvP1 fvP2 vA; subst.
-      have ?:= tree_fv_step_cut eA; subst.
-      have {IH} //= [|[sy y]/=[ys [+ H4]]]:= IH _ erefl sIgn _ fvP2 (valid_tree_step vA eA).
-        by apply/fsubset_trans/fvP1/vars_tree_step_cut/eA.
-      have H5 := step_cb_same_subst1 vA eA; subst.
-      have [x[tl[H1 [H2 H3]]]] := s2l_CutBrothers s1 nilC vA eA.
-      rewrite H1 H2 H5 => -[???]; subst.
-      repeat eexists; by apply CutE.
-    + move=> s1 s2 r A B n fv fv' ? eA rB IH s4 ? sIgn fvP1 fvP2 vA; subst. 
+    + have [fvB fvs] := vars_tree_step_sub_flow vtA vts1 eA.
       have /=vB:= (valid_tree_step vA eA). 
+      have [[sy y][ys /=[+ {}IH]]]:= IH _ erefl s0 fvB fvs vB.
+      have /=[] := path_atom_exp_cut pA eA => ?; subst.
+        have H5 := step_cb_same_subst1 vA eA; subst.
+        have [x[tl[H1 [H2 H3]]]] := s2l_CutBrothers s1 nilC vA eA.
+        rewrite H1 H2 H5 => -[???]; subst.
+        have ?:= tree_fv_step_cut eA; subst.
+        by repeat eexists; apply: CutE => //=.
       have fA := step_not_failed eA notF.
       have [s[x[xs +]]] := failed_t2l vA fA s1 nilC.
-      move=> H; rewrite H; repeat eexists.
-      have [fvB fvs] := vars_tree_step_sub_flow fvP1 fvP2 eA.
-      have [[sy y][ys /=[+ {}IH]]]:= IH _ erefl sIgn fvB fvs vB.
+      move=> H Hx; rewrite H; repeat eexists.
       case: x H => [|g gs].
         fNilG => H.
         have [] := s2l_empty_hd_success vA (step_not_failed eA notF) H.
@@ -44,21 +41,20 @@ Section NurEqiv.
       fConsG g gs.
       case: g => [[|c] ca] H; last first.
         have:= s2l_Expanded_call vA eA H.
-        move=> []?; subst.
-        case X: bc => /=[fv2 rules] ? fB ; subst => /=.
-        case: rules X => [|r0 rs] X Hx; rewrite Hx; subst.
-          by move=> ->; apply: FailE X _.
+        move=> [??]; subst; move: IH.
+        case X: bc => /=[fv3 rules] IH fB ; subst => /=.
+        case: rules X => [|r0 rs] X; rewrite Hx.
+          by move=> <-; apply: FailE X _.
         move=> [???]; subst.
         rewrite cats0 in IH.
         by apply: CallE X _.
       have [[[? SS] H1]] := s2l_Expanded_cut vA eA H; subst.
-      rewrite cats0 => ->[???]; subst.
+      rewrite cats0 Hx => -[???]; subst.
       by apply: CutE.
-    + move=> s1 s2 A B r n fv ? fA nA H IH s3 ? sIgn fvP1 fvP2 vA; subst.
-      have vB := valid_tree_next_alt vA nA.
+    + have vB := valid_tree_next_alt vA nA.
       have H1 := failed_next_alt_some_t2l _ vA fA nA.
-      have {}fvP := vars_tree_next_alt_sub_flow fvP1 nA.
-      have {IH} /= [[sx x][xs [H2 H3]]] := IH _ erefl sIgn fvP fvP2 vB.
+      have {}fvP := vars_tree_next_alt_sub_flow vtA nA.
+      have {IH} /= [[sx x][xs [H2 H3]]] := IH _ erefl s0 fvP vts1 vB.
       by rewrite H1; eauto.
   Qed.
   Print Assumptions tree_to_elpi.
@@ -101,23 +97,20 @@ Proof.
         have:= next_cut_s2l fA' vA' H X => /=.
         rewrite clean_ca_nil/= => -[H1 H2].
         have /= [t1[n [fv0[{}IH H3]]]] := IH _ _ (valid_tree_step vA' X) H1; subst.
-        move: H2; case: ifP => Hx [??]; subst.
-          repeat eexists.
-          apply: run_fail fA nA _.
-          apply: run_cut X IH.
-        repeat eexists.
-        apply: run_fail fA nA _.
-        apply: run_step X IH.
+        move: H2; case: ifP => Hx [??]; subst;
+        repeat eexists; apply: run_fail fA nA _;
+        apply: run_step (X) erefl IH.
+          by apply: path_atom_cut X.
+        by apply: path_atom_exp X.
       rewrite -(@clean_ca_nil (t2l _ _ _)) in H.
       case X: (step u p fv s A) => [[fv' r'] A'].
       have:= next_cut_s2l fA vA H X => /=.
       rewrite clean_ca_nil/= => -[H1 H2].
       have /= [t1[n[fv0[{}IH H3]]]] := IH _ _ (valid_tree_step vA X) H1; subst.
-      move: H2; case: ifP => Hx [??]; subst.
-        repeat eexists.
-        by apply: run_cut IH.
-      repeat eexists.
-      by apply: run_step IH.
+      move: H2; case: ifP => Hx [??]; subst;
+      repeat eexists; apply: run_step (X) erefl IH.
+        by apply: path_atom_cut X.
+      by apply: path_atom_exp X.
     }
   - move=> s1 s2 a [s0 r0]/= rs gl r t ca fv fv' B ELPI IH s3 A vA H.
     {
@@ -134,13 +127,15 @@ Proof.
         have /= [t1[n[fv0[{}IH ?]]]] := IH _ _ (valid_tree_step vA' erefl) H1; subst.
         repeat eexists.
         apply: run_fail fA nA _.
-        apply: run_step H2 IH.
+        apply: run_step (H2) erefl IH.
+        apply: path_atom_exp H2.
       rewrite -(@clean_ca_nil (t2l _ _ _)) in H.
       have [] := next_callS_s2l p u fv fA vA H.
       rewrite B/= clean_ca_nil/= => H1 H2.
       have /= [t1[n [?[{}IH ?]]]] := IH _ _ (valid_tree_step vA erefl) H1; subst.
       repeat eexists.
-      apply: run_step H2 IH.
+      apply: run_step (H2) erefl IH.
+      apply: path_atom_exp H2.
     }
   - move=> s1 s2 s3 t gl a al r ca fv fv' B ELPI IH s4 A vA H.
     {
@@ -157,13 +152,15 @@ Proof.
         have /= [t1[n[?[{}IH ?]]]] := IH _ _ (valid_tree_step vA' erefl) H1; subst.
         repeat eexists.
         apply: run_fail fA nA _.
-        apply: run_step H2 IH.
+        apply: run_step (H2) erefl IH.
+        apply: path_atom_exp H2.
       rewrite -(@clean_ca_nil (t2l _ _ _)) in H.
       have [] := next_callS_s2l p u fv fA vA H.
       rewrite B/= clean_ca_nil/=cat0s => H1 H2.
       have /= [t1[n[?[{}IH ?]]]] := IH _ _ (valid_tree_step vA erefl) H1; subst.
       repeat eexists.
-      apply: run_step H2 IH.
+      apply: run_step (H2) erefl IH.
+      apply: path_atom_exp H2.
     }
 Qed.
 
